Progress using eqmRinverses on monadstate, I think we might need to generalize the inverses lemmas

theories/Basics/MonadState.v
@@ -36,14 +36,6 @@ Section State.
   Definition stateT (s : typ) (m : typ -> typ) (a : typ) : typ :=
     s ~~> m (prod_typ s a).
 
-
-  Lemma prod_eq_rel :
-    forall {A B : typ}, S × A ≡ S ⊗ A.
-  Proof.
-    repeat intro; split; repeat intro; destruct x, y; cbn in *;
-      destruct H; split; assumption.
-  Qed.
-
   Global Instance EqmR_stateT : EqmR (stateT S m).
   econstructor. Unshelve. 2 : {
     refine (
@@ -56,17 +48,15 @@ Section State.
   - rewrite H0.
     assert (forall s : S, eqmR (S × A) @ (x @ s, y @ s)). {
       intros. eapply eqmR_Proper_mono; eauto.
-      apply prod_eq_rel.
+      apply prod_rel_eq.
     }
     pose proof eqmR_equal.
     eapply H2 in H1. cbn in H1.
     apply H1.
   - eapply eqmR_Proper_mono; eauto.
     2 : { eapply eqmR_equal in H. 2 : reflexivity. apply H. }
-    apply prod_eq_rel.
+    apply prod_rel_eq.
   Defined.
-
-
 
   Global Instance EqmR_OK_stateT : EqmR_OK (stateT S m).
   Proof.
@@ -131,59 +121,176 @@ Section State.
       apply prod_rel_monotone. intuition. eauto.
   Qed.
 
-  (* ret and bind definition for stateT. *)
-  Instance stateT_Monad : Monad typ_proper (stateT S m).
-  constructor.
-  - intros. unfold stateT. refine (-=->! (fun x => _) _).
-    Unshelve. 2 : {
-      refine (-=->! (fun s => ret @ (s, x)) _).
-      repeat intro. rewrite H. reflexivity.
-    }
+  (* Making properness proofs opaque, so it's doesn't do the ugly unfolding in
+   proof contexts *)
+  Lemma Proper_ret :
+    forall (a : typ) (x : a),
+      Proper (equalE S ==> equalE (m (S × a))) (fun s : S => ret @ (s, x)).
+  Proof.
+    repeat intro. rewrite H. reflexivity.
+  Qed.
+
+  Lemma Proper_ret_2 :
+    forall (a : typ),
+      Proper (equalE a ==> equalE (S ~~> m (S × a)))
+         (fun x : a => (-=->!) (fun s : S => ret @ (s, x)) (Proper_ret a x)).
+  Proof.
     repeat intro. cbn. rewrite H0, H. reflexivity.
-  - unfold stateT. intros.
-    refine (-=->! (fun k => _) _).
-    Unshelve. 2 : {
-      refine (-=->! (fun x => _) _).
-      Unshelve. 2 : {
-        pose proof (uncurry f).
-        assert ((S × a) -=-> m (S × b)). {
-          refine (-=->! (fun y => _) _).
-          Unshelve. 2 : {
-            destruct y. pose proof (X @ (t0, t)). eauto.
-          }
-          repeat intro. destruct x0, y. cbn.
-          destruct H. cbn in *. rewrite H, H0. reflexivity.
-        }
-        pose proof (bind X0).
-        pose proof (k @ x).
-        apply (X1 @ X2).
-      }
-      repeat intro. unfold uncurry. cbn. rewrite H.
-      reflexivity.
-    }
+  Qed.
+
+  Lemma Proper_bind:
+    forall (a b : typ) (f : a -=-> stateT S m b),
+      S ~~> m (S × a) ->
+      S ->
+      Proper (equalE (S × a) ==> equalE (m (S × b)))
+              (fun y : S * a => uncurry f @ (snd y, fst y)).
+  Proof.
+    repeat intro.
+    destruct x, y. cbn.
+    destruct H. cbn in *. rewrite H, H0. reflexivity.
+  Defined.
+
+  Lemma Proper_bind_2:
+    forall (a b : typ) (f : a -=-> stateT S m b) (k : S ~~> m (S × a)),
+      Proper (equalE S ==> equalE (m (S × b)))
+          (fun x : S =>
+            let X :=
+                (-=->!) (fun y : S * a => uncurry f @ (snd y, fst y))
+                        (Proper_bind a b f k x) in
+            @bind typ typ_proper m Mm (S × a) (S × b) X @ (k @ x)).
+  Proof.
+    repeat intro. unfold uncurry. cbn. unfold Proper_bind.
+    rewrite H.
+    reflexivity.
+  Qed.
+
+  Lemma Proper_bind_3:
+    forall (a b : typ) (f : a -=-> stateT S m b),
+      @Proper (S ~~> m (S × a) -> S ~~> m (S × b))
+              (equalE (S ~~> m (S × a)) ==> equalE (S ~~> m (S × b)))
+              (fun k : S ~~> m (S × a) =>
+                  (-=->!)
+                    (fun x : S =>
+                      let X :=
+                          (-=->!)
+                            (fun y : S * a =>
+                                @uncurry a S (m (S × b)) f @ (@snd S a y, @fst S a y))
+                            (Proper_bind a b f k x) in
+                      @bind typ typ_proper m Mm (S × a) (S × b) X @ (k @ x))
+                    (Proper_bind_2 a b f k)).
+  Proof.
+    intros a b f. unfold Proper_bind.
     repeat intro. unfold uncurry. cbn. rewrite H.
     rewrite H0. reflexivity.
+  Qed.
+
+  Set Transparent Obligations.
+  (* ret and bind definition for stateT. *)
+  Program Instance stateT_Monad : Monad typ_proper (stateT S m).
+  Next Obligation.
+  intros. unfold stateT. refine (-=->! (fun x => _) _).
+  Unshelve. 2 : {
+      refine (-=->! (fun s => ret @ (s, x)) _). apply Proper_ret.
+  } apply Proper_ret_2.
+  Defined.
+  Next Obligation.
+  unfold stateT. intros.
+  refine (-=->! (fun k => _) _).
+  Unshelve. 2 : {
+    refine (-=->! (fun x => _) _).
+    Unshelve. 2 : {
+      assert ((S × a) -=-> m (S × b)). {
+        refine (-=->! (fun y => uncurry f @ (snd y, fst y)) _).
+        apply Proper_bind; eauto.
+      }
+      exact ((bind X) @ (k @ x)).
+    }
+      apply Proper_bind_2; eauto.
+  }
+  apply Proper_bind_3; eauto.
+  Defined.
+
+  Lemma relate_state_proper:
+    forall (A1 : typ) (R : relationH A1 A1),
+      Proper (equalE ((S × A1) × (S × A1)) ==> equalE prop_typ)
+             (fun p : S * A1 * (S * A1) =>
+                fst (fst p) == fst (snd p) /\ R @ (snd (fst p), snd (snd p))).
+  Proof.
+    repeat intro. destruct x, y. destruct t, t0, t1, t2. cbn.
+    split; intro.
+    destruct H. cbn in H, H1. destruct H, H0, H1.
+    split. rewrite <- H. rewrite <- H1. auto.
+    rewrite <- H2. rewrite <- H4. auto.
+    destruct H. cbn in H, H1. destruct H, H0, H1.
+    split. rewrite H. rewrite H1. auto.
+    rewrite H2. rewrite H4. auto.
+  Qed.
+
+  Program Definition relate_state {A1 : typ} (R : relationH A1 A1) : relationH (S × A1) (S × A1).
+  refine (-=->! (fun (p : (S * A1) * (S * A1)) => fst (fst p) == fst (snd p) /\ R @ (snd (fst p), snd (snd p))) _).
+  apply relate_state_proper; auto.
   Defined.
 
 
-  (* Lemma ret_ok :  forall {A1 A2} (RA : A1 -> A2 -> Prop) (a1:A1) (a2:A2), *)
-  (*     RA a1 a2 -> (eqmR RA (ret a1) (ret a2)). *)
-  (* Proof. *)
-  (*   unfold eqmR, EqmR_stateT. *)
-  (*   intros. *)
-  (*   repeat red. apply eqmR_ret. assumption. *)
-  (*   constructor; auto. *)
-  (* Qed. *)
+  Lemma relate_state_Symmetric {A1 : typ} (R : relationH A1 A1)
+        (RH: SymmetricH R): SymmetricH (relate_state R).
+  Proof.
+    repeat intro. cbn. destruct p. destruct t, t0. destruct H.
+    cbn in *. split. symmetry; auto. apply SymmetricH_Symmetric in RH.
+    apply RH. apply H0.
+  Qed.
+
+  Lemma relate_state_Transitive {A1 : typ} (R : relationH A1 A1)
+        (RH: TransitiveH R) : TransitiveH (relate_state R).
+  Proof.
+    repeat intro. cbn. destruct p. destruct t, t0. destruct H.
+    cbn in *. destruct H0, H1. destruct q, p, p0. cbn in *. split.
+    rewrite <- H0. rewrite <- H1. apply H.
+    apply TransitiveH_Transitive in RH.
+    eapply RH. apply H2. rewrite H4. apply H3.
+  Qed.
 
   Instance EqmRMonad_stateT (HS: inhabited S) : @EqmRMonad (stateT S m) _ _.
   Proof.
   constructor.
   - repeat intro; cbn. pose proof (eqmR_ret _ _ _ _ H).
     assert (s == s) by reflexivity.
-    (* repeat.r *)
-    (* pose proof eqmR_rel_prod. *)
-    (* specialize (H2 _ _ _ _ _ _ _ S RA). *)
-    (* eapply eqmR_rel_prod; eauto. *)
+    eapply eqmR_ret; eauto. cbn. split; eauto.
+  - repeat intro.
+    change (eqmR (S ⊗ RB) @ (((bind kb1 @ ma1) @ s), ((bind kb2 @ ma2) @ s))).
+    eapply eqmR_bind_ProperH; eauto.
+    intros. destruct a1 as (s1 & a1).
+    cbn in H.
+    pose proof eqmR_mayRet_l as Heq.
+    specialize (Heq _ _ _ _ _ _ (ma1 @ s) (ma2 @ s) (S ⊗ RA) (H s) _ H2).
+    edestruct Heq as (x & SRA & Hmr).
+    exists x. clear Heq.
+    split; eauto. split; eauto.
+    cbn. destruct x as (s2 & a2). cbn.
+    destruct SRA as (Seq & Aeq). cbn in Seq, Aeq.
+    rewrite Seq in *. clear Seq.
+    + specialize (H0 a1).
+      assert (Hma: mayRet (stateT S m) ma1 @ a1). {
+        cbn. intros. cbn in H2.
+        specialize (H2 (S ⊗ R)).
+        assert (SymmetricH (S ⊗ R)). {
+          apply SymmetricH_Symmetric.
+          eapply prod_rel_sym. repeat intro. rewrite H3. reflexivity.
+          apply SymmetricH_Symmetric. apply HS0. }
+        assert (TransitiveH (S ⊗ R)). {
+          apply TransitiveH_Transitive.
+          eapply prod_rel_trans. repeat intro. rewrite H4. auto.
+          apply TransitiveH_Transitive. auto. }
+        specialize (H2 H3 H4 (EQ s)). cbn in H2. apply H2.
+      }
+      specialize (H0 Hma).
+      edestruct H0 as (a2' & HRA & Hmr' & Heqm); clear H0.
+      specialize (H1 a2' Hmr').
+      edestruct H1 as (a1' & HRA' & Hmr'' & Heqm'); clear H1.
+      (* IY: Need to generalize EqmRMonadInverses lemmas to EqmR? *)
+  Admitted.
+
+
   (* - repeat intro. *)
   (*   change (eqmR (S ⊗ RB) @ (((bind kb1 @ ma1) @ s), ((bind kb2 @ ma2) @ s))). *)
   (*   pose proof eqmR_rel_prod. *)
